Separate out definition of graphs.

FOL/Structure.thy
@@ -1,5 +1,5 @@
 theory Structure
-imports Set
+imports Graph
 begin
 
 section {* Components of a structure *}
@@ -16,67 +16,19 @@ definition target :: "i \<Rightarrow> i" where [rewrite]:
 definition graph :: "i \<Rightarrow> i" where [rewrite]:
   "graph(\<Gamma>)  = fst(snd(snd(\<Gamma>)))"
 
-section {* Graphs *}
-
-definition is_graph :: "i \<Rightarrow> o" where [rewrite]:
-  "is_graph(G) \<longleftrightarrow> (\<forall>x\<in>G. x = \<langle>fst(x),snd(x)\<rangle>)"
-
-lemma is_graphE [forward]: "is_graph(G) \<Longrightarrow> x \<in> G \<Longrightarrow> x = \<langle>fst(x),snd(x)\<rangle>" by auto2
-setup {* del_prfstep_thm_eqforward @{thm is_graph_def} *}
-
-definition gr_source :: "i \<Rightarrow> i" where [rewrite]:
-  "gr_source(G) = {fst(p). p \<in> G}"
-lemma gr_sourceI [typing2]: "\<langle>a,b\<rangle> \<in> G \<Longrightarrow> a \<in> gr_source(G)" by auto2
-lemma gr_sourceE [forward]: "is_graph(G) \<Longrightarrow> a \<in> gr_source(G) \<Longrightarrow> \<exists>b. \<langle>a,b\<rangle>\<in>G" by auto2
-setup {* del_prfstep_thm @{thm gr_source_def} *}
-
-definition gr_target :: "i \<Rightarrow> i" where [rewrite]:
-  "gr_target(G) = {snd(p). p \<in> G}"
-lemma gr_targetI [typing2]: "\<langle>a,b\<rangle> \<in> G \<Longrightarrow> b \<in> gr_target(G)" by auto2
-lemma gr_targetE [forward]: "is_graph(G) \<Longrightarrow> b \<in> gr_target(G) \<Longrightarrow> \<exists>a. \<langle>a,b\<rangle>\<in>G" by auto2
-setup {* del_prfstep_thm @{thm gr_target_def} *}
-
-definition gr_field :: "i \<Rightarrow> i" where [rewrite]:
-  "gr_field(G) = gr_source(G) \<union> gr_target(G)"
-lemma gr_fieldI1 [typing2]: "\<langle>a,b\<rangle> \<in> G \<Longrightarrow> a \<in> gr_field(G)" by auto2
-lemma gr_fieldI2 [typing2]: "\<langle>a,b\<rangle> \<in> G \<Longrightarrow> b \<in> gr_field(G)" by auto2
-
-definition gr_id :: "i \<Rightarrow> i" where [rewrite]:
-  "gr_id(A) = {\<langle>a,a\<rangle>. a \<in> A}"
-lemma gr_id_is_graph [forward]: "is_graph(gr_id(A))" by auto2
-lemma gr_idI [typing2]: "a \<in> A \<Longrightarrow> \<langle>a,a\<rangle> \<in> gr_id(A)" by auto2
-lemma gr_id_iff [rewrite]: "p \<in> gr_id(A) \<longleftrightarrow> (p\<in>A\<times>A \<and> fst(p) = snd(p))" by auto2
-setup {* del_prfstep_thm @{thm gr_id_def} *}
-
-definition gr_comp :: "i \<Rightarrow> i \<Rightarrow> i"  (infixr "\<circ>\<^sub>g" 60) where [rewrite]:
-  "s \<circ>\<^sub>g r = {p\<in>gr_source(r)\<times>gr_target(s). \<exists>z. \<langle>fst(p),z\<rangle>\<in>r \<and> \<langle>z,snd(p)\<rangle>\<in>s}"
-
-lemma gr_comp_is_graph [forward]: "is_graph(s \<circ>\<^sub>g r)" by auto2
-lemma gr_compI [backward1, backward2]:
-  "\<langle>x,y\<rangle> \<in> r \<Longrightarrow> \<langle>y,z\<rangle> \<in> s \<Longrightarrow> \<langle>x,z\<rangle> \<in> s \<circ>\<^sub>g r" by auto2
-lemma gr_compE [forward]:
-  "p \<in> s \<circ>\<^sub>g r \<Longrightarrow> \<exists>y. \<langle>fst(p),y\<rangle> \<in> r \<and> \<langle>y,snd(p)\<rangle> \<in> s" by auto2
-setup {* del_prfstep_thm @{thm gr_comp_def} *}
-
 section {* Evaluation function: shared by families and functions *}
 
 definition feval :: "i \<Rightarrow> i \<Rightarrow> i" (infixl "`" 90) where [rewrite]:
-  "f ` x = (THE y. \<langle>x,y\<rangle> \<in> graph(f))"
+  "f ` x = graph_eval(graph(f),x)"
 setup {* register_wellform_data ("f ` x", ["x \<in> source(f)"]) *}
 setup {* add_prfstep_check_req ("f ` x", "x \<in> source(f)") *}
-
-definition is_func_graph :: "i \<Rightarrow> i \<Rightarrow> o" where [rewrite]:
-  "is_func_graph(G,X) \<longleftrightarrow> (\<forall>a\<in>X. \<exists>!y. \<langle>a,y\<rangle> \<in> G)"
-  
-definition func_graphs :: "i \<Rightarrow> i \<Rightarrow> i" where [rewrite]:
-  "func_graphs(X,Y) = {G\<in>Pow(X\<times>Y). is_func_graph(G,X)}"
 
 section {* Families *}
 
 (* Predicate for families. *)
 definition is_family :: "i \<Rightarrow> o" where [rewrite]:
   "is_family(F) \<longleftrightarrow> (let G = graph(F) in let S = source(F) in
-     is_graph(G) \<and> gr_source(G) \<subseteq> S \<and> is_func_graph(G,S) \<and> F = \<langle>S,\<emptyset>,G,\<emptyset>\<rangle>)"
+     is_func_graph(G,S) \<and> F = \<langle>S,\<emptyset>,G,\<emptyset>\<rangle>)"
 
 (* Constructor for families. *)
 definition Tup :: "i \<Rightarrow> (i \<Rightarrow> i) \<Rightarrow> i" where [rewrite]:
@@ -91,7 +43,8 @@ lemma Tup_eval [rewrite]: "a \<in> source(Tup(I,f)) \<Longrightarrow> Tup(I,f) `
 
 (* Equality on families. *)
 lemma family_eq [backward]:
-  "is_family(f) \<Longrightarrow> is_family(g) \<Longrightarrow> source(f) = source(g) \<Longrightarrow> \<forall>a\<in>source(f). f`a = g`a \<Longrightarrow> f = g" by auto2
+  "is_family(f) \<Longrightarrow> is_family(g) \<Longrightarrow> source(f) = source(g) \<Longrightarrow> \<forall>a\<in>source(f). f`a = g`a \<Longrightarrow> f = g"
+@proof @have "\<forall>a\<in>source(f). graph_eval(graph(f),a) = graph_eval(graph(g),a)" @qed
 
 (* Pi space is the space of families with values in specified sets.
    Need to use Sigma(I,B) to construct the set. *)
