FOL/Graph.thy
@@ -1,0 +1,73 @@
+theory Graph
+  imports Set
+begin
+
+section {* Graphs *}
+
+definition is_graph :: "i \<Rightarrow> o" where [rewrite]:
+  "is_graph(G) \<longleftrightarrow> (\<forall>x\<in>G. x = \<langle>fst(x),snd(x)\<rangle>)"
+
+lemma is_graphE [forward]: "is_graph(G) \<Longrightarrow> x \<in> G \<Longrightarrow> x = \<langle>fst(x),snd(x)\<rangle>" by auto2
+setup {* del_prfstep_thm_eqforward @{thm is_graph_def} *}
+
+definition gr_source :: "i \<Rightarrow> i" where [rewrite]:
+  "gr_source(G) = {fst(p). p \<in> G}"
+lemma gr_sourceI [typing2]: "\<langle>a,b\<rangle> \<in> G \<Longrightarrow> a \<in> gr_source(G)" by auto2
+lemma gr_sourceE [forward]: "is_graph(G) \<Longrightarrow> a \<in> gr_source(G) \<Longrightarrow> \<exists>b. \<langle>a,b\<rangle>\<in>G" by auto2
+setup {* del_prfstep_thm @{thm gr_source_def} *}
+
+definition gr_target :: "i \<Rightarrow> i" where [rewrite]:
+  "gr_target(G) = {snd(p). p \<in> G}"
+lemma gr_targetI [typing2]: "\<langle>a,b\<rangle> \<in> G \<Longrightarrow> b \<in> gr_target(G)" by auto2
+lemma gr_targetE [forward]: "is_graph(G) \<Longrightarrow> b \<in> gr_target(G) \<Longrightarrow> \<exists>a. \<langle>a,b\<rangle>\<in>G" by auto2
+setup {* del_prfstep_thm @{thm gr_target_def} *}
+
+definition gr_field :: "i \<Rightarrow> i" where [rewrite]:
+  "gr_field(G) = gr_source(G) \<union> gr_target(G)"
+lemma gr_fieldI1 [typing2]: "\<langle>a,b\<rangle> \<in> G \<Longrightarrow> a \<in> gr_field(G)" by auto2
+lemma gr_fieldI2 [typing2]: "\<langle>a,b\<rangle> \<in> G \<Longrightarrow> b \<in> gr_field(G)" by auto2
+
+definition gr_id :: "i \<Rightarrow> i" where [rewrite]:
+  "gr_id(A) = {\<langle>a,a\<rangle>. a \<in> A}"
+lemma gr_id_is_graph [forward]: "is_graph(gr_id(A))" by auto2
+lemma gr_idI [typing2]: "a \<in> A \<Longrightarrow> \<langle>a,a\<rangle> \<in> gr_id(A)" by auto2
+lemma gr_id_iff [rewrite]: "p \<in> gr_id(A) \<longleftrightarrow> (p\<in>A\<times>A \<and> fst(p) = snd(p))" by auto2
+setup {* del_prfstep_thm @{thm gr_id_def} *}
+
+definition gr_comp :: "i \<Rightarrow> i \<Rightarrow> i"  (infixr "\<circ>\<^sub>g" 60) where [rewrite]:
+  "s \<circ>\<^sub>g r = {p\<in>gr_source(r)\<times>gr_target(s). \<exists>z. \<langle>fst(p),z\<rangle>\<in>r \<and> \<langle>z,snd(p)\<rangle>\<in>s}"
+
+lemma gr_comp_is_graph [forward]: "is_graph(s \<circ>\<^sub>g r)" by auto2
+lemma gr_compI [backward1, backward2]:
+  "\<langle>x,y\<rangle> \<in> r \<Longrightarrow> \<langle>y,z\<rangle> \<in> s \<Longrightarrow> \<langle>x,z\<rangle> \<in> s \<circ>\<^sub>g r" by auto2
+lemma gr_compE [forward]:
+  "p \<in> s \<circ>\<^sub>g r \<Longrightarrow> \<exists>y. \<langle>fst(p),y\<rangle> \<in> r \<and> \<langle>y,snd(p)\<rangle> \<in> s" by auto2
+setup {* del_prfstep_thm @{thm gr_comp_def} *}
+
+section \<open>Evaluation on a graph\<close>
+
+definition is_func_graph :: "i \<Rightarrow> i \<Rightarrow> o" where [rewrite]:
+  "is_func_graph(G,X) \<longleftrightarrow> is_graph(G) \<and> gr_source(G) \<subseteq> X \<and> (\<forall>a\<in>X. \<exists>!y. \<langle>a,y\<rangle> \<in> G)"
+  
+definition func_graphs :: "i \<Rightarrow> i \<Rightarrow> i" where [rewrite]:
+  "func_graphs(X,Y) = {G\<in>Pow(X\<times>Y). is_func_graph(G,X)}"
+
+definition graph_eval :: "i \<Rightarrow> i \<Rightarrow> i" where [rewrite]:
+  "graph_eval(G,x) = (THE y. \<langle>x,y\<rangle> \<in> G)"
+
+lemma is_func_graphD [forward]:
+  "is_func_graph(G,X) \<Longrightarrow> is_graph(G) \<and> gr_source(G) \<subseteq> X" by auto2
+
+lemma is_func_graphD2 [forward]:
+  "is_func_graph(G,X) \<Longrightarrow> x \<in> X \<Longrightarrow> \<langle>x, graph_eval(G,x)\<rangle> \<in> G" by auto2
+
+lemma is_func_graphD3 [forward,backward2]:
+  "is_func_graph(G,X) \<Longrightarrow> \<langle>x,y\<rangle> \<in> G \<Longrightarrow> x \<in> X \<Longrightarrow> graph_eval(G,x) = y" by auto2
+
+lemma graph_eq [backward1]:
+  "is_func_graph(G,X) \<Longrightarrow> is_func_graph(H,X) \<Longrightarrow>
+   \<forall>x\<in>X. graph_eval(G,x) = graph_eval(H,x) \<Longrightarrow> G = H" by auto2
+setup {* del_prfstep_thm_eqforward @{thm is_func_graph_def} *}
+setup {* del_prfstep_thm @{thm graph_eval_def} *}
+
+end
